theories/bij.v
@@ -41,7 +41,7 @@ Lemma card_bij (A B: finType) (f : bij A B) : #|A| = #|B|.
 Proof. exact: (bij_card_eq (f := f)). Qed.
 Arguments card_bij [A B] f.
 
-Lemma bij_mem_imset (aT rT : finType) (f : bij aT rT) (x : aT) (A : {set aT}): 
+Lemma bij_imset_f (aT rT : finType) (f : bij aT rT) (x : aT) (A : {set aT}): 
   (f x \in [set f x | x in A]) = (x \in A).
 Proof. 
   apply/imsetP/idP; last by exists x.
@@ -50,7 +50,7 @@ Qed.
 
 Lemma bij_imsetC (aT rT : finType) (f : bij aT rT) (A : {set aT}) : 
   ~: [set f x | x in A] = [set f x | x in ~: A].
-Proof. apply/setP => x. by rewrite -[x](bijK' f) !inE !bij_mem_imset inE. Qed.
+Proof. apply/setP => x. by rewrite -[x](bijK' f) !inE !bij_imset_f inE. Qed.
 
 Lemma bij_eqLR (aT rT : finType) (f : bij aT rT) x y : 
   (f x == y) = (x == f^-1 y).
